pass

Iris/Iris/Instances/Lib/GhostMap.lean
@@ -7,30 +7,30 @@ Authors: Сухарик (@suhr)
 module
 
 public import Iris.Instances.IProp
-public import Iris.Std.HeapInstances
 public import Iris.BI.Lib.Fractional
-public import Iris.Algebra.BigOp
-public import Iris.BI.BigOp.BigOp
+public import Iris.ProofMode
 
 namespace Iris
 
-open Iris Std HeapView PartialMap Iris.Algebra CMRA BI
+open Iris Std HeapView PartialMap Iris.Algebra CMRA BI ProofMode
 
-class GhostMapG (GF : BundledGFunctors) (F: outParam (Type _))
-    (K V: Type _)(H : outParam <| Type _ → Type _)
+class GhostMapG (GF : BundledGFunctors) (F : outParam (Type _))
+    (K V : Type _) (H : outParam <| Type _ → Type _)
     [UFraction F] [LawfulFiniteMap H K] where
-  elem: ElemG GF (constOF (HeapView F K (Agree (LeibnizO V)) H))
+  elem : ElemG GF (constOF (HeapView F K (Agree (LeibnizO V)) H))
+
+attribute [reducible, instance] GhostMapG.elem
 
 section definitions
 
-variable [UFraction F][LawfulFiniteMap H K][hgm: GhostMapG GF F K V H]
+variable [UFraction F] [LawfulFiniteMap H K] [GhostMapG GF F K V H]
 
-public def ghost_map_auth (γ : GName) (dq : DFrac F) (m : H V): IProp GF :=
-  iOwn (E := hgm.elem) γ
+public def ghost_map_auth (γ : GName) (dq : DFrac F) (m : H V) : IProp GF :=
+  iOwn (E := GhostMapG.elem) γ
     (Auth dq (Iris.Std.PartialMap.map (fun x ↦ toAgree ⟨x⟩) m))
 
-public def ghost_map_elem (γ : GName) (dq : DFrac F) (k: K) (v: V): IProp GF :=
-  iOwn (E := hgm.elem) γ (Frag k dq (toAgree ⟨v⟩))
+public def ghost_map_elem (γ : GName) (dq : DFrac F) (k : K) (v : V) : IProp GF :=
+  iOwn (E := GhostMapG.elem) γ (Frag k dq (toAgree ⟨v⟩))
 
 end definitions
 
@@ -42,20 +42,21 @@ notation γ " ↪◯MAP[" k "] " v => ghost_map_elem γ (DFrac.own 1) k v
 section lemmas
 
 variable (F K V : Type _) (H : Type _ → Type _) [UFraction F] [LawfulFiniteMap H K]
-variable [hgm: GhostMapG GF F K V H]
+variable [hgm : GhostMapG GF F K V H]
 
 @[rocq_alias ghost_map_elem_timeless]
-instance (γ : GName)(k: K)(dq: DFrac F)(v: V): Timeless (PROP := IProp GF) (γ ↪◯MAP[k]{dq} v) :=
-  iOwn_timeless (E := hgm.elem)
+instance (γ : GName) (k : K) (dq : DFrac F) (v : V) : Timeless (PROP := IProp GF) (γ ↪◯MAP[k]{dq} v) := by
+  unfold ghost_map_elem
+  infer_instance
 
 @[rocq_alias ghost_map_elem_persistent]
-instance (γ : GName)(k: K)(v: V): Persistent (PROP := IProp GF) (γ ↪◯MAP[k]{.discard} v) := by
+instance (γ : GName) (k : K) (v : V): Persistent (PROP := IProp GF) (γ ↪◯MAP[k]{.discard} v) := by
   unfold ghost_map_elem
   infer_instance
 
 @[rocq_alias ghost_map_elem_fractional]
-instance ghost_map_elem_fractional (γ : GName)(k: K)(v: V)
-    : Fractional (PROP := IProp GF) (fun q: F => γ ↪◯MAP[k]{.own q} v) where
+instance ghost_map_elem_fractional (γ : GName) (k : K) (v : V)
+    : Fractional (PROP := IProp GF) (fun q : F => γ ↪◯MAP[k]{.own q} v) where
   fractional p q := by
     -- If using `refine`/`apply` instead of stating facts with `have`,
     -- it's possible to eliminate some of implicit annotations.
@@ -67,7 +68,7 @@ instance ghost_map_elem_fractional (γ : GName)(k: K)(v: V)
     exact Agree.idemp.symm
 
 @[rocq_alias ghost_map_elem_as_fractional]
-instance (γ : GName) (k: K) (v: V)
+instance (γ : GName) (k : K) (v : V)
     : AsFractional (PROP := IProp GF) (γ ↪◯MAP[k]{.own q} v)
       (fun q => γ ↪◯MAP[k]{.own q} v) q where
   as_fractional := IProp.ext_iff.mp rfl
@@ -88,20 +89,15 @@ theorem ghost_map_elems_unseal γ (m : H V) dq :
     sorry
 
 @[rocq_alias ghost_map_elem_valid]
-theorem ghost_map_elem_valid (γ : GName) (k : K) (dq: DFrac F) (v: V) :
+theorem ghost_map_elem_valid (γ : GName) (k : K) (dq : DFrac F) (v : V) :
     (γ ↪◯MAP[k]{dq} v) ⊢@{IProp GF} internalCmraValid dq := by
   refine (iOwn_cmraValid (E := hgm.elem)).trans ?_
   iintro h
   ipure h; ipure_intro
   exact (frag_valid_iff.mp h).left
 
-#check iOwn_op
-#check frag_op_valid_iff
-#check Iris.Agree.op
-#check toAgree_op_valid_iff_eq
-
 @[rocq_alias ghost_map_elem_valid_2]
-theorem ghost_map_elem_valid_2 (γ : GName) (k : K) (dq1: DFrac F) (dq2: DFrac F) (v1: V) (v2: V) :
+theorem ghost_map_elem_valid_2 (γ : GName) (k : K) (dq1 dq2 : DFrac F) (v1 v2 : V) :
     (γ ↪◯MAP[k]{dq1} v1) ∗ (γ ↪◯MAP[k]{dq2} v2) ⊢@{IProp GF}
       internalCmraValid (dq1 • dq2) ∧ ⌜v1 = v2⌝ := by
   -- To use `iOwn_*` family of lemmas in the proof mode,
@@ -115,7 +111,7 @@ theorem ghost_map_elem_valid_2 (γ : GName) (k : K) (dq1: DFrac F) (dq2: DFrac F
   exact ⟨vdq, congrArg (·.car) (toAgree_op_valid_iff_eq.mp va)⟩
 
 @[rocq_alias ghost_map_elem_agree]
-theorem ghost_map_elem_agree (γ : GName) (k : K) (dq1 : DFrac F) (dq2 : DFrac F) (v1 : V) (v2 : V) :
+theorem ghost_map_elem_agree (γ : GName) (k : K) (dq1 dq2 : DFrac F) (v1 v2 : V) :
     (γ ↪◯MAP[k]{dq1} v1) ∗ (γ ↪◯MAP[k]{dq2} v2) ⊢@{IProp GF} ⌜v1 = v2⌝ := by
   -- Notation difference with the Rocq version: if you have a hypothesis of shape `H : A ∧ B`,
   -- in Iris you can't derive both `H1 : A` and `H2 : B` at the same time,
@@ -124,18 +120,18 @@ theorem ghost_map_elem_agree (γ : GName) (k : K) (dq1 : DFrac F) (dq2 : DFrac F
   iintro H
   icases ghost_map_elem_valid_2 $$ H with ⟨-, $⟩
 
--- Global Instance ghost_map_elem_combine_gives γ k v1 dq1 v2 dq2 :
---   CombineSepGives (γ ↪◯MAP[k]{dq1} v1) (γ ↪◯MAP[k]{dq2} v2)
---     ⌜✓ (dq1 • dq2) ∧ v1 = v2⌝ := sorry
-
-#check frag_op_equiv
-#check BI.equiv_iff
-#check Agree.op
-#check Agree.toAgree_op_valid_iff_equiv
-#check View.frag_ne
+@[rocq_alias ghost_map_elem_combine_gives]
+instance ghost_map_elem_combine_gives γ (k : K) (dq1 dq2 : DFrac F) (v1 v2 : V) :
+  CombineSepGives (PROP := IProp GF)
+    (γ ↪◯MAP[k]{dq1} v1) (γ ↪◯MAP[k]{dq2} v2)
+    iprop(⌜✓ (dq1 • dq2) ∧ v1 = v2⌝) where
+  combine_sep_gives := by
+    iintro H
+    icases ghost_map_elem_valid_2 $$ H with %H
+    imodintro; ipure_intro; assumption
 
 @[rocq_alias ghost_map_elem_combine]
-theorem ghost_map_elem_combine (γ : GName) (k : K) (dq1 : DFrac F) (dq2 : DFrac F) (v1 : V) (v2 : V) :
+theorem ghost_map_elem_combine (γ : GName) (k : K) (dq1 dq2 : DFrac F) (v1 v2 : V) :
     (γ ↪◯MAP[k]{dq1} v1) ∗ (γ ↪◯MAP[k]{dq2} v2)
     ⊢@{IProp GF} (γ ↪◯MAP[k]{dq1 • dq2} v1) ∗ ⌜v1 = v2⌝ := by
   iintro H
@@ -153,12 +149,18 @@ theorem ghost_map_elem_combine (γ : GName) (k : K) (dq1 : DFrac F) (dq2 : DFrac
   refine OFE.NonExpansive.eqv ?_
   exact Agree.idemp.symm
 
--- Global Instance ghost_map_elem_combine_as (γ : GName) (k : K) (dq1 : DFrac F) (dq2 : DFrac F) (v1 : V) (v2 : V) :
---   CombineSepAs (γ ↪◯MAP[k]{dq1} v1) (γ ↪◯MAP[k]{dq2} v2)
---                 (γ ↪◯MAP[k]{dq1 • dq2} v1) | 60 := sorry
+@[rocq_alias ghost_map_elem_combine_as]
+instance ghost_map_elem_combine_as (γ : GName) (k : K) (dq1 dq2 : DFrac F) (v1 v2 : V) :
+  CombineSepAs (PROP := IProp GF)
+    (γ ↪◯MAP[k]{dq1} v1) (γ ↪◯MAP[k]{dq2} v2)
+    (γ ↪◯MAP[k]{dq1 • dq2} v1) where
+  combine_sep_as := by
+    iintro H
+    icases ghost_map_elem_combine $$ H with ⟨H, -⟩
+    iframe
 
 @[rocq_alias ghost_map_elem_frac_ne]
-theorem ghost_map_elem_frac_ne γ (k1 : K) (k2 : K) (dq1 : DFrac F) (dq2 : DFrac F) (v1 : V) (v2 : V) :
+theorem ghost_map_elem_frac_ne γ (k1 k2 : K) (dq1 dq2 : DFrac F) (v1 v2 : V) :
    ¬ ✓ (dq1 • dq2) →
      (γ ↪◯MAP[k1]{dq1} v1) ∗ (γ ↪◯MAP[k2]{dq2} v2) ⊢@{IProp GF} ⌜k1 ≠ k2⌝ := by
   iintro %Hcontra H
@@ -171,61 +173,106 @@ theorem ghost_map_elem_frac_ne γ (k1 : K) (k2 : K) (dq1 : DFrac F) (dq2 : DFrac
   · ipure_intro; exact Heq
 
 @[rocq_alias ghost_map_elem_ne]
-theorem ghost_map_elem_ne γ (k1 : K) (k2 : K) (dq2 : DFrac F) (v1 : V) (v2 : V) :
-  ⊢@{IProp GF} (γ ↪◯MAP[k1] v1) -∗ (γ ↪◯MAP[k2]{dq2} v2) -∗ ⌜k1 ≠ k2⌝ := sorry
+theorem ghost_map_elem_ne γ (k1 k2 : K) (dq : DFrac F) (v1 v2 : V) :
+  ⊢@{IProp GF} (γ ↪◯MAP[k1] v1) -∗ (γ ↪◯MAP[k2]{dq} v2) -∗ ⌜k1 ≠ k2⌝ := by
+  iintro H G
+  iapply ghost_map_elem_frac_ne $$ [$H $G]
+  intro HContra
+  exact Fraction.Whole.not_fractional UFraction.one_whole (DFrac.valid_own_op HContra)
 
 --  Make an element read-only.
 theorem ghost_map_elem_persist (γ : GName) (k : K) (dq : DFrac F) (v : V) :
-  ⊢@{IProp GF} (γ ↪◯MAP[k]{dq} v) ==∗ (γ ↪◯MAP[k]{.discard} v) := sorry
+  ⊢@{IProp GF} (γ ↪◯MAP[k]{dq} v) ==∗ (γ ↪◯MAP[k]{.discard} v) := by
+  unfold ghost_map_elem
+  iintro H
+  iapply iOwn_update (E := hgm.elem) $$ H
+  exact update_frag_discard
 
 --  Recover fractional ownership for read-only element.
-theorem ghost_map_elem_unpersist (γ : GName) (k : K) (v : V) :
-  ⊢@{IProp GF} (γ ↪◯MAP[k]{.discard} v) ==∗ ∃ q, (γ ↪◯MAP[k]{.own q} v) := sorry
+theorem ghost_map_elem_unpersist [IsSplitFraction F] (γ : GName) (k : K) (v : V) :
+  ⊢@{IProp GF} (γ ↪◯MAP[k]{.discard} v) ==∗ ∃ q, (γ ↪◯MAP[k]{.own q} v) := by
+  unfold ghost_map_elem
+  iintro H
+  imod iOwn_updateP (E := hgm.elem) update_frag_acquire $$ H with ⟨%a, %Heq, G⟩
+  obtain ⟨q, Heq⟩ := Heq
+  iexists q; subst Heq
+  iframe
 
 -- * lemmas about [ghost_map_auth]
 
 @[rocq_alias ghost_map_alloc_strong]
 theorem ghost_map_alloc_strong (P : GName → Prop) (m : H V) :
-  (hP : ∀ N, ∃ k, N ≤ k ∧ P k) →
-  ⊢@{IProp GF} |==> ∃ γ, ⌜P γ⌝ ∗ (γ ↪●MAP m) ∗ [∗map] k ↦ v ∈ m, γ ↪◯MAP[k] v := sorry
+  (∀ N, ∃ k, N ≤ k ∧ P k) →
+  ⊢@{IProp GF} |==> ∃ γ, ⌜P γ⌝ ∗ (γ ↪●MAP m) ∗ [∗map] k ↦ v ∈ m, γ ↪◯MAP[k] v := by
+  unfold ghost_map_elem ghost_map_auth
+  iintro %Hinf
+  imod iOwn_alloc_strong (E := hgm.elem)
+    (HeapView.Auth (DFrac.own 1) (Std.PartialMap.map (fun x => toAgree ⟨x⟩) ∅)) P Hinf with ⟨%γ, %HP, G⟩
+  · rw [auth_valid_iff]
+    exact DFrac.valid_own_one
+  · iexists γ; iframe %HP
+    -- missing upstream: gmap_view_alloc_big
+    sorry
 
 @[rocq_alias ghost_map_alloc_strong_empty]
 theorem ghost_map_alloc_strong_empty (P : GName → Prop) :
-  (hP : ∀ N, ∃ k, N ≤ k ∧ P k) →
-  ⊢@{IProp GF} |==> ∃ γ, ⌜P γ⌝ ∗ (γ ↪●MAP (∅ : H V)) := sorry
+  (∀ N, ∃ k, N ≤ k ∧ P k) →
+  ⊢@{IProp GF} |==> ∃ γ, ⌜P γ⌝ ∗ (γ ↪●MAP (∅ : H V)) := by
+  iintro %Hinf
+  imod ghost_map_alloc_strong _ _ _ _ P (∅ : H V) Hinf with ⟨%γ, H1, H2, -⟩
+  iexists γ
+  iframe
 
 @[rocq_alias ghost_map_alloc]
 theorem ghost_map_alloc (m : H V) :
-    ⊢@{IProp GF} |==> ∃ γ, (γ ↪●MAP m) ∗
-      [∗map] k ↦ v ∈ m, γ ↪◯MAP[k] v := sorry
+  ⊢@{IProp GF} |==> ∃ γ, (γ ↪●MAP m) ∗
+    [∗map] k ↦ v ∈ m, γ ↪◯MAP[k] v := by
+
+  sorry
 
 @[rocq_alias ghost_map_alloc_empty]
 theorem ghost_map_alloc_empty :
-  ⊢@{IProp GF} |==> ∃ γ, (γ ↪●MAP (∅ : H V)) := sorry
+  ⊢@{IProp GF} |==> ∃ γ, (γ ↪●MAP (∅ : H V)) := by
+
+  sorry
 
 -- Global Instance ghost_map_auth_timeless γ dq m :
 @[rocq_alias ghost_map_auth_timeless]
-instance (m : H V): BI.Timeless (PROP := IProp GF) (γ ↪●MAP{dq} m) := sorry
+instance (m : H V): Timeless (PROP := IProp GF) (γ ↪●MAP{dq} m) := by
+  unfold ghost_map_auth
+  infer_instance
 
 @[rocq_alias ghost_map_persistent]
-instance (m : H V): BI.Timeless (PROP := IProp GF) (γ ↪●MAP{.discard} m) := sorry
+instance (m : H V): Timeless (PROP := IProp GF) (γ ↪●MAP{.discard} m) := by
+  unfold ghost_map_auth
+  infer_instance
 
 @[rocq_alias ghost_map_auth_fractional]
-instance (m : H V): Fractional (PROP := IProp GF) (fun q => γ ↪●MAP{.own q} m) := sorry
+instance ghost_map_auth_fractional (m : H V): Fractional (PROP := IProp GF) (fun q => γ ↪●MAP{.own q} m) where
+  fractional p q := by
+    unfold ghost_map_auth
+    refine .trans ?_ (iOwn_op (E := hgm.elem))
+    refine equiv_iff.mp ?_
+    refine .trans ?_ ((iOwn_ne (E := hgm.elem)).eqv auth_dfrac_op_equiv)
+    rfl
 
--- Global Instance ghost_map_auth_as_fractional γ q m :
---   AsFractional (γ ↪●MAP{.own q} m) (λ q, γ ↪●MAP{.own q} m)%I q := sorry
+@[rocq_alias ghost_map_auth_as_fractional]
+instance (γ : GName) (m : H V) (q : F)
+    : AsFractional (PROP := IProp GF) (γ ↪●MAP{.own q} m)
+      (fun q => γ ↪●MAP{.own q} m) q where
+  as_fractional := IProp.ext_iff.mp rfl
+  as_fractional_fractional := ghost_map_auth_fractional F K V H m
 
 @[rocq_alias ghost_map_auth_valid]
 theorem ghost_map_auth_valid γ (dq : DFrac F) (m : H V) :
   ⊢@{IProp GF} (γ ↪●MAP{dq} m) -∗ ⌜✓ dq⌝ := sorry
 
 @[rocq_alias ghost_map_auth_valid_2]
-theorem ghost_map_auth_valid_2 γ (dq1 : DFrac F) (dq2 : DFrac F) (m1 : H V) (m2 : H V) :
+theorem ghost_map_auth_valid_2 γ (dq1 dq2 : DFrac F) (m1 m2 : H V) :
   ⊢@{IProp GF} (γ ↪●MAP{dq1} m1) -∗ (γ ↪●MAP{dq2} m2) -∗ ⌜✓ (dq1 • dq2) ∧ m1 = m2⌝ := sorry
 
 @[rocq_alias ghost_map_auth_agree]
-theorem ghost_map_auth_agree γ (dq1 : DFrac F) (dq2 : DFrac F) (m1 : H V) (m2 : H V) :
+theorem ghost_map_auth_agree γ (dq1 dq2 : DFrac F) (m1 m2 : H V) :
   ⊢@{IProp GF} (γ ↪●MAP{dq1} m1) -∗ (γ ↪●MAP{dq2} m2) -∗ ⌜m1 = m2⌝ := sorry
 
 @[rocq_alias ghost_map_auth_persist]
@@ -242,28 +289,42 @@ theorem ghost_map_auth_unpersist γ (m : H V) :
 theorem ghost_map_lookup {γ dq} {m : H V} {k : K} {dq' v} :
   ⊢@{IProp GF} (γ ↪●MAP{dq} m) -∗ (γ ↪◯MAP[k]{dq'} v) -∗ ⌜get? m k = some v⌝ := sorry
 
--- Global Instance ghost_map_lookup_combine_gives_1 {γ dq m k dq' v} :
---   CombineSepGives (γ ↪●MAP{dq} m) (γ ↪◯MAP[k]{dq'} v) ⌜get? m k = .some v⌝ := sorry
+@[rocq_alias ghost_map_lookup_combine_gives_1]
+instance ghost_map_lookup_combine_gives_1 γ (m : H V) (k : K) (dq1 dq2 : DFrac F) (v : V) :
+  CombineSepGives (PROP := IProp GF)
+    (γ ↪●MAP{dq1} m) (γ ↪◯MAP[k]{dq2} v)
+    iprop(⌜get? m k = .some v⌝) where
+  combine_sep_gives := by
+    iintro ⟨H, G⟩
+    icases ghost_map_lookup $$ H G with %H
+    imodintro; ipure_intro; assumption
 
--- Global Instance ghost_map_lookup_combine_gives_2 {γ dq m k dq' v} :
---   CombineSepGives (γ ↪◯MAP[k]{dq} v) (γ ↪●MAP{dq'} m) ⌜get? m k = .some v⌝ := sorry
+@[rocq_alias ghost_map_lookup_combine_gives_2]
+instance ghost_map_lookup_combine_gives_2 γ (m : H V) (k : K) (dq dq' : DFrac F) (v : V) :
+  CombineSepGives (PROP := IProp GF)
+    (γ ↪◯MAP[k]{dq} v) (γ ↪●MAP{dq'} m)
+    iprop(⌜get? m k = .some v⌝) where
+  combine_sep_gives := by
+    iintro ⟨H, G⟩
+    icases ghost_map_lookup $$ G H with %H
+    imodintro; ipure_intro; assumption
 
 @[rocq_alias ghost_map_insert]
-theorem ghost_map_insert {γ} {m: H V} (k: K) (v: V) :
-  get? m k = None →
+theorem ghost_map_insert {γ} {m : H V} (k : K) (v : V) :
+  get? m k = .none →
   ⊢@{IProp GF} (γ ↪●MAP m) ==∗ (γ ↪●MAP insert m k v) ∗ γ ↪◯MAP[k] v := sorry
 
 @[rocq_alias ghost_map_insert_persist]
-theorem ghost_map_insert_persist {γ} {m: H V} (k: K) (v: V) :
-  get? m k = None →
+theorem ghost_map_insert_persist {γ} {m : H V} (k : K) (v : V) :
+  get? m k = .none →
   ⊢@{IProp GF} (γ ↪●MAP m) ==∗ (γ ↪●MAP insert m k v) ∗ (γ ↪◯MAP[k]{.discard} v) := sorry
 
 @[rocq_alias ghost_map_delete]
-theorem ghost_map_delete {γ} {m: H V} (k: K) (v: V) :
+theorem ghost_map_delete {γ} {m : H V} (k : K) (v : V) :
   ⊢@{IProp GF} (γ ↪●MAP m) -∗ (γ ↪◯MAP[k] v) ==∗ γ ↪●MAP delete m k := sorry
 
 @[rocq_alias ghost_map_update]
-theorem ghost_map_update {γ} {m: H V} (k: K) (v: V) (w: V) :
+theorem ghost_map_update {γ} {m : H V} (k : K) (v : V) (w : V) :
   ⊢@{IProp GF} (γ ↪●MAP m) -∗ (γ ↪◯MAP[k] v) ==∗ (γ ↪●MAP insert m k w) ∗ γ ↪◯MAP[k] w := sorry
 
 --  Big-op versions of above lemmas
